\bexo
The Forward Euler's Method is defined by the recurence relation:
\begin{equation}
	\tb{S}_{k+1}=\left(
	[\tb{I}_2]+\Delta t[\bs{\alpha}]
	\right)\tb{S}_k.
\end{equation}
Compute the first three steps $\tb{S}_1$, $\tb{S}_2$ and $\tb{S}_3$ of Forward Euler's Method for 
\begin{equation}
	[\bs{\alpha}]=\begin{bmatrix}
		0 & -\omega_0^2 \\ 1 &0
	\end{bmatrix} \esp \tb{S}_0=\begin{Bmatrix}
		1\\0
	\end{Bmatrix}
\end{equation}
\eexo 



\solution{
\begin{equation}
\tb{S}_1=\begin{Bmatrix}
	1\\\Delta t
\end{Bmatrix} \esp 
\tb{S}_2=\begin{Bmatrix}
	1-\omega_0^2\Delta  t^2\\ 2\Delta t
\end{Bmatrix}\esp
\tb{S}_2=\begin{Bmatrix}
	1-3\omega_0^2\Delta  t^2\\ \Delta t
	\left(3-\omega_0^2\Delta  t^2
	\right)
\end{Bmatrix}.
\end{equation}}



