\bexo
What is the solution of  
\begin{equation}
	m\ddot{x}(t)+c\ddot{x}(t)+kx(t)=F\cos(\omega t),
\end{equation}
with 
\begin{equation}
	x(0)=0,\, \dot{x}(0)=0.
\end{equation}

\eexo
\solution{


\begin{equation}
	\ddot{x}(t)+\mu\ddot{x}(t)+\omega_0^2 x(t)=F'\cos(\omega t)\esp F'=\dfrac{F}{m}\esp \mu=\dfrac{c}{m}.
\end{equation}


The particular solution 
\begin{equation}
	x_p(t)=A\cos(\omega t)+B\sin(\omega t).
\end{equation}


\begin{equation}
	(\omega^2_0-\omega^2)(A\cos(\omega t)+B\sin(\omega t))+\omega \mu (-A\sin(\omega t)+B\cos(\omega t))=F'\cos(\omega t).
\end{equation}


\begin{equation}
	\left[
		\begin{array}{cc}
		{\omega^2_0-\omega^2m}&{\omega \mu}\\
		{-\omega \mu}&{\omega^2_0-\omega^2}
	\end{array}
	\right]\left\{
	\begin{array}{c}
		{A}\\
		{B}
	\end{array}
	\right\}=\left\{
	\begin{array}{c}
		{F'}\\
		{0}
	\end{array}
	\right\}
\end{equation}

A necessary condition 

\begin{equation}
	(\omega^2_0-\omega^2)^2+\omega^2\mu^2 >0
\end{equation}

\begin{equation}
	A=\dfrac{F'(\omega^2_0-\omega^2 )}{(\omega^2_0-\omega^2)^2+\omega^2\mu^2} \esp B=\dfrac{F'\omega \mu}{(\omega^2_0-\omega^2)^2+\omega^2\mu^2} 
\end{equation}

\begin{equation}
	x_p(t)=\dfrac{F'}{\sqrt{(\omega^2_0-\omega^2)^2+\omega^2\mu^2}}\left(
	\cos(\phi)
	\cos(\omega t)+\sin(\phi) \sin(\omega t)
	\right)
\end{equation}
with
\begin{equation}
	\cos(\phi)=\dfrac{\omega^2_0-\omega^2}{\sqrt{(\omega^2_0-\omega^2)^2+\omega^2\mu^2}} \esp
	\sin(\phi)=\dfrac{\omega \mu}{\sqrt{(\omega^2_0-\omega^2)^2+\omega^2\mu^2}}
\end{equation}

\begin{equation}
	x_p(t)=\dfrac{F'}{\sqrt{(k-\omega^2m)^2+\omega^2c^2}}
	\cos(\omega t-\phi)
\end{equation}



\begin{equation}
	\ddot{x}(t)+\mu\ddot{x}(t)+\omega_0^2 x(t)=0, x(t)=exp(-\alpha t)
\end{equation}



}
