\bexo
We are considering the harmonic damped oscillator\footnote{oscillator harmonique amorti} of a mass $m$ linked to a rigid support by a spring\footnote{ressort} $k$. An external force $f(t)$ can be applied to this dynamical system. Hence the displacement $x(t)$ of the mass is governed by
\begin{equation}
	m\ddot{x}(t)+kx(t)=f(t).
\end{equation}
The numerical values of the parameters are 
\begin{equation}
	m=1 \esp k=1.
\end{equation}
At time $t=0$ , the initial condition of the system are
\begin{equation}
	x(0)=0\esp \dot{x}(0)=1.
\end{equation}
at time $t=1$, a constant force $f=-1$ is applied to the mass. 

\begin{itemize}
	\item What is the expression of the displacement $x(t)$ ?
\end{itemize}



%\begin{figure}[h]
%\begin{center}
%\begin{tikzpicture}
%\path (-40mm,0);
%\node[mass] at (2.4,0) {};
%\draw[spring] (0,0.5) -- (1.65,0.5); 
%\draw [damper] (0,-0.5) -- (1.65,-0.5);
%% Rigid body
%\draw[thick] (0,-1.5) -- (0,1.2);
%\fill [pattern = north east lines] (-0.3,-1.5) rectangle (0,1.2);
%\node[text width=5cm] at (3.2,0.1) {$k$};
%\node[text width=5cm] at (3.2,-1) {$c$};
%\node[text width=5cm] at (4.6,1) {$m$};
%\node[text width=5cm] at (4.6,-1) {$x(t)$};
%% Force under the mass
%\draw [thick] (2.2,-1.4) -- (2.2,-1.2);
%\draw [thick, ->] (2.2,-1.4) -- (2.7,-1.4);
%\node[text width=5cm] at (4.5,-1.7) {$M f(t)$};
%\end{tikzpicture}
%\end{center}
%\end{figure}



\eexo
\solution{


\begin{equation}
	\ddot{x}(t)+\mu\ddot{x}(t)+\omega_0^2 x(t)=F'\cos(\omega t)\esp F'=\dfrac{F}{m}\esp \mu=\dfrac{c}{m}.
\end{equation}


The particular solution 
\begin{equation}
	x_p(t)=A\cos(\omega t)+B\sin(\omega t).
\end{equation}


\begin{equation}
	(\omega^2_0-\omega^2)(A\cos(\omega t)+B\sin(\omega t))+\omega \mu (-A\sin(\omega t)+B\cos(\omega t))=F'\cos(\omega t).
\end{equation}


\begin{equation}
	\left[
		\begin{array}{cc}
		{\omega^2_0-\omega^2m}&{\omega \mu}\\
		{-\omega \mu}&{\omega^2_0-\omega^2}
	\end{array}
	\right]\left\{
	\begin{array}{c}
		{A}\\
		{B}
	\end{array}
	\right\}=\left\{
	\begin{array}{c}
		{F'}\\
		{0}
	\end{array}
	\right\}
\end{equation}

A necessary condition 

\begin{equation}
	(\omega^2_0-\omega^2)^2+\omega^2\mu^2 >0
\end{equation}

\begin{equation}
	A=\dfrac{F'(\omega^2_0-\omega^2 )}{(\omega^2_0-\omega^2)^2+\omega^2\mu^2} \esp B=\dfrac{F'\omega \mu}{(\omega^2_0-\omega^2)^2+\omega^2\mu^2} 
\end{equation}

\begin{equation}
	x_p(t)=\dfrac{F'}{\sqrt{(\omega^2_0-\omega^2)^2+\omega^2\mu^2}}\left(
	\cos(\phi)
	\cos(\omega t)+\sin(\phi) \sin(\omega t)
	\right)
\end{equation}
with
\begin{equation}
	\cos(\phi)=\dfrac{\omega^2_0-\omega^2}{\sqrt{(\omega^2_0-\omega^2)^2+\omega^2\mu^2}} \esp
	\sin(\phi)=\dfrac{\omega \mu}{\sqrt{(\omega^2_0-\omega^2)^2+\omega^2\mu^2}}
\end{equation}

\begin{equation}
	x_p(t)=\dfrac{F'}{\sqrt{(k-\omega^2m)^2+\omega^2c^2}}
	\cos(\omega t-\phi)
\end{equation}



\begin{equation}
	\ddot{x}(t)+\mu\ddot{x}(t)+\omega_0^2 x(t)=0, x(t)=exp(-\alpha t)
\end{equation}



}
