\bexo
Let consider polynomial  
\begin{equation}
	P(X)=X^3+(1+j)X^2+(-6+j)X-6j \esp j=\sqrt{1}.
\end{equation}
\begin{itemize}
	\item Show that $-j$ is a root of $P$.
	\item Find the two other roots.
\end{itemize} 
 
\eexo
\solution{
\begin{align}
	P(j)&=j-(1+j)-j(-6+j)-6j=j-1-j+6j+1-6j=0
\end{align}




$-j$ is then one root of the polynomial. It is then possible to factorize $P$ by $(X+j)$. This can be done by two means. \\

The first one is euclidian division
\begin{equation}
	\begin{array}{rrrrrrrrrr|l}
	        &{X^3}&{+}&{(1+j)}&{X^2}&{+}&{(-6+j)}&{X}&{-}&{6j}&{X+j}\\	\cline{11-11} 
\od{-}&	     {X^3}&{+}&{j}    &{X^2}&   &        &   &   &    &{X^2+X-6}\\ \cline{1-10} 
      &           &   &       &{X^2}&{+}&{(-6+j)}&{X}&{-}&{6j}\\
\od{-}&           &   &       &{X^2}&{+}&{j}&{X}&&\\    \cline{5-10} 
      &           &   &       &     &{}&{-6}&{X}&-&6j\\  
 \od{-}           &           &   &       &     &{}&{-6}&{X}&-&6j\\ \cline{7-10} 
       &           &   &       &     &{}&{}&{}&&\tb{0}\\           
	\end{array}
\end{equation}


The second method is the identification 

\begin{align}
	X^3+(1+j)X^2+(-6+j)X-6j&=(X+j)(aX^2+bX+c)\\
	&=aX^3+(b+ja)X^2+(c+bj)X+cj
\end{align}
By identification of the coefficients in $X^3$:
\begin{equation}
	a=1.
\end{equation}
By identification of the coefficients in $X^2$:
\begin{equation}
	b+ja=1+j \so b=1.
\end{equation}
By identification of the coefficients in $X$:
\begin{equation}
	c+bj=-6+j \so c=-6.
\end{equation}
We can check that this value of $c$ is ok and leads to an identification of the term of zero order. 
\begin{equation}
	c+bj=-6+j \so c=-6.
\end{equation}

The two other roots of out polynomial are the one of $X^2+X-6$. Once more, two methods to find the result. \\

The first one is the classical one
\begin{equation}
	\Delta=1^2+4\times 6=25=5^2
\end{equation}

The two roots are then
\begin{equation}
	\dfrac{-1\pm\sqrt{\Delta}}{2}\so X=2 \tr{ and } X=-3.
\end{equation}

The second method corresponds to the formula
\begin{equation}
	(X-x_1)(X-x_2)=X^2-(x_1+x_2)X+x_1x_2
\end{equation}
Hence $x_1+x_2=-1$ and $x_1x_2=-6$. The two roots are then $x_1=2$ and $x_2=-3$.

}